Make math, temporal, and collections libraries work with Dafny 3.0.0

ironfleet/src/Dafny/Distributed/Common/Logic/Temporal/Time.i.dfy
@@ -19,737 +19,737 @@ import opened Math__mul_auto_i
 // DEFINITIONS
 /////////////////////////
 
-    function{:opaque} earliestStepWithin(start:int, x:temporal, span:int, timefun:imap<int, int>):int
-        requires imaptotal(timefun);
-        requires monotonic_from(start, timefun);
-        requires sat(start, eventuallywithin(x, span, timefun));
-        ensures  sat(earliestStepWithin(start, x, span, timefun), beforeabsolutetime(x, timefun[start] + span, timefun));
-        ensures  start <= earliestStepWithin(start, x, span, timefun);
-        ensures  forall i :: start <= i < earliestStepWithin(start, x, span, timefun) ==> !sat(i, x);
-    {
-        TemporalAssist();
-        var i1 := earliestStep(start, x);
-        var i2 := earliestStep(start, beforeabsolutetime(x, timefun[start] + span, timefun));
-        assert TLe(i1, i2);
-        i1
-    }
+function{:opaque} earliestStepWithin(start:int, x:temporal, span:int, timefun:imap<int, int>):int
+  requires imaptotal(timefun)
+  requires monotonic_from(start, timefun)
+  requires sat(start, eventuallywithin(x, span, timefun))
+  ensures  sat(earliestStepWithin(start, x, span, timefun), beforeabsolutetime(x, timefun[start] + span, timefun))
+  ensures  start <= earliestStepWithin(start, x, span, timefun)
+  ensures  forall i :: start <= i < earliestStepWithin(start, x, span, timefun) ==> !sat(i, x)
+{
+  TemporalAssist();
+  var i1 := earliestStep(start, x);
+  var i2 := earliestStep(start, beforeabsolutetime(x, timefun[start] + span, timefun));
+  assert TLe(i1, i2);
+  i1
+}
 
-    function{:opaque} earliestActionWithin(start:int, x:temporal, span:int, timefun:imap<int, int>):int
-        requires imaptotal(timefun);
-        requires monotonic_from(start, timefun);
-        requires sat(start, eventuallynextwithin(x, span, timefun));
-        ensures  sat(earliestActionWithin(start, x, span, timefun), and(x, next(before(timefun[start] + span, timefun))));
-        ensures  start <= earliestActionWithin(start, x, span, timefun);
-        ensures  forall i :: start <= i < earliestActionWithin(start, x, span, timefun) ==> !sat(i, x);
-    {
-        TemporalAssist();
-        var i1 := earliestStep(start, x);
-        var i2 := earliestStep(start, and(x, next(before(timefun[start] + span, timefun))));
-        assert TLe(i1, i2);
-        i1
-    }
+function{:opaque} earliestActionWithin(start:int, x:temporal, span:int, timefun:imap<int, int>):int
+  requires imaptotal(timefun)
+  requires monotonic_from(start, timefun)
+  requires sat(start, eventuallynextwithin(x, span, timefun))
+  ensures  sat(earliestActionWithin(start, x, span, timefun), and(x, next(before(timefun[start] + span, timefun))))
+  ensures  start <= earliestActionWithin(start, x, span, timefun)
+  ensures  forall i :: start <= i < earliestActionWithin(start, x, span, timefun) ==> !sat(i, x)
+{
+  TemporalAssist();
+  var i1 := earliestStep(start, x);
+  var i2 := earliestStep(start, and(x, next(before(timefun[start] + span, timefun))));
+  assert TLe(i1, i2);
+  i1
+}
 
-    function{:opaque} goalOrDecrease(goal:temporal, d:imap<int, int>, span:int, timefun:imap<int, int>):temporal
-        requires imaptotal(d);
-        requires imaptotal(timefun);
-        ensures  forall i {:trigger sat(i, goalOrDecrease(goal, d, span, timefun))} :: sat(i, goalOrDecrease(goal, d, span, timefun)) <==>
-                    sat(i, eventuallywithin(or(goal, stepDecrease(i, d)), span, timefun));
-    {
-        TemporalAssist();
-        stepmap(imap i :: sat(i, eventuallywithin(or(goal, stepDecrease(i, d)), span, timefun)))
-    }
+function{:opaque} goalOrDecrease(goal:temporal, d:imap<int, int>, span:int, timefun:imap<int, int>):temporal
+  requires imaptotal(d)
+  requires imaptotal(timefun)
+  ensures  forall i {:trigger sat(i, goalOrDecrease(goal, d, span, timefun))} :: sat(i, goalOrDecrease(goal, d, span, timefun)) <==>
+               sat(i, eventuallywithin(or(goal, stepDecrease(i, d)), span, timefun))
+{
+  TemporalAssist();
+  stepmap(imap i :: sat(i, eventuallywithin(or(goal, stepDecrease(i, d)), span, timefun)))
+}
 
-    function{:opaque} nextOrDecreaseWithin(goal:temporal, d:imap<int, int>, span:int, timefun:imap<int, int>):temporal
-        requires imaptotal(d);
-        requires imaptotal(timefun);
-        ensures  forall i {:trigger sat(i, nextOrDecreaseWithin(goal, d, span, timefun))} :: sat(i, nextOrDecreaseWithin(goal, d, span, timefun)) <==>
-                    sat(i, eventuallynextwithin(or(goal, nextDecrease(i, d)), span, timefun));
-    {
-        TemporalAssist();
-        stepmap(imap i :: sat(i, eventuallynextwithin(or(goal, nextDecrease(i, d)), span, timefun)))
-    }
+function{:opaque} nextOrDecreaseWithin(goal:temporal, d:imap<int, int>, span:int, timefun:imap<int, int>):temporal
+  requires imaptotal(d)
+  requires imaptotal(timefun)
+  ensures  forall i {:trigger sat(i, nextOrDecreaseWithin(goal, d, span, timefun))} :: sat(i, nextOrDecreaseWithin(goal, d, span, timefun)) <==>
+               sat(i, eventuallynextwithin(or(goal, nextDecrease(i, d)), span, timefun));
+{
+  TemporalAssist();
+  stepmap(imap i :: sat(i, eventuallynextwithin(or(goal, nextDecrease(i, d)), span, timefun)))
+}
 
-    function{:opaque} eventuallywithinspans(d:imap<int, int>, goal:temporal, span:int, timefun:imap<int, int>):temporal
-        requires imaptotal(d);
-        requires imaptotal(timefun);
-        ensures  forall i {:trigger sat(i, eventuallywithinspans(d, goal, span, timefun))} ::
-                    sat(i, eventuallywithinspans(d, goal, span, timefun)) <==>
-                    sat(i, eventuallywithin(goal, span * d[i], timefun));
-    {
-        TemporalAssist();
-        stepmap(imap i :: sat(i, eventuallywithin(goal, span * d[i], timefun)))
-    }
+function{:opaque} eventuallywithinspans(d:imap<int, int>, goal:temporal, span:int, timefun:imap<int, int>):temporal
+  requires imaptotal(d)
+  requires imaptotal(timefun)
+  ensures  forall i {:trigger sat(i, eventuallywithinspans(d, goal, span, timefun))} ::
+               sat(i, eventuallywithinspans(d, goal, span, timefun)) <==>
+               sat(i, eventuallywithin(goal, span * d[i], timefun));
+{
+  TemporalAssist();
+  stepmap(imap i :: sat(i, eventuallywithin(goal, span * d[i], timefun)))
+}
 
-    function{:opaque} eventuallynextwithinspans(d:imap<int, int>, goal:temporal, span:int, timefun:imap<int, int>):temporal
-        requires imaptotal(d);
-        requires imaptotal(timefun);
-        ensures  forall i {:trigger sat(i, eventuallynextwithinspans(d, goal, span, timefun))} ::
-                    sat(i, eventuallynextwithinspans(d, goal, span, timefun)) <==>
-                    sat(i, eventuallynextwithin(goal, span * d[i], timefun));
-    {
-        TemporalAssist();
-        stepmap(imap i :: sat(i, eventuallynextwithin(goal, span * d[i], timefun)))
-    }
+function{:opaque} eventuallynextwithinspans(d:imap<int, int>, goal:temporal, span:int, timefun:imap<int, int>):temporal
+  requires imaptotal(d)
+  requires imaptotal(timefun)
+  ensures  forall i {:trigger sat(i, eventuallynextwithinspans(d, goal, span, timefun))} ::
+               sat(i, eventuallynextwithinspans(d, goal, span, timefun)) <==>
+               sat(i, eventuallynextwithin(goal, span * d[i], timefun));
+{
+  TemporalAssist();
+  stepmap(imap i :: sat(i, eventuallynextwithin(goal, span * d[i], timefun)))
+}
 
-    function stepattimeboundary(i:int, j:int, t:int, timefun:imap<int, int>):int
-        requires imaptotal(timefun);
-        requires monotonic_from(i, timefun);
-        requires timefun[i] <= t;
-        requires timefun[j] >= t;
-        requires i <= j;
-        ensures  var k := stepattimeboundary(i, j, t, timefun);
-                    timefun[k] <= t
-                 && i <= k <= j
-                 && forall m :: m > k ==> timefun[m] >= t;
-        decreases j-i;
-    {
-        if i == j then i else if timefun[j-1] <= t then j-1 else stepattimeboundary(i, j-1, t, timefun)
-    }
+function stepattimeboundary(i:int, j:int, t:int, timefun:imap<int, int>):int
+  requires imaptotal(timefun)
+  requires monotonic_from(i, timefun)
+  requires timefun[i] <= t
+  requires timefun[j] >= t
+  requires i <= j
+  ensures  var k := stepattimeboundary(i, j, t, timefun);
+           && timefun[k] <= t
+           && i <= k <= j
+           && forall m :: m > k ==> timefun[m] >= t
+  decreases j-i
+{
+  if i == j then i else if timefun[j-1] <= t then j-1 else stepattimeboundary(i, j-1, t, timefun)
+}
 
 /////////////////////////
 // LEMMAS
 /////////////////////////
 
-    lemma TemporalEventuallyWithin(i:int, j:int, x:temporal, span:int, timefun:imap<int, int>)
-        requires imaptotal(timefun);
-        requires i <= j;
-        requires sat(j, beforeabsolutetime(x, timefun[i] + span, timefun));
-        ensures  sat(i, eventuallywithin(x, span, timefun));
-    {
-        TemporalAssist();
-    }
+lemma TemporalEventuallyWithin(i:int, j:int, x:temporal, span:int, timefun:imap<int, int>)
+  requires imaptotal(timefun)
+  requires i <= j
+  requires sat(j, beforeabsolutetime(x, timefun[i] + span, timefun))
+  ensures  sat(i, eventuallywithin(x, span, timefun))
+{
+  TemporalAssist();
+}
 
-    lemma TemporalEventuallyNextWithin(i:int, j:int, x:temporal, span:int, timefun:imap<int, int>)
-        requires imaptotal(timefun);
-        requires i <= j;
-        requires sat(j, x);
-        requires sat(j+1, before(timefun[i] + span, timefun));
-        ensures  sat(i, eventuallynextwithin(x, span, timefun));
-    {
-        TemporalAssist();
-    }
+lemma TemporalEventuallyNextWithin(i:int, j:int, x:temporal, span:int, timefun:imap<int, int>)
+  requires imaptotal(timefun)
+  requires i <= j
+  requires sat(j, x)
+  requires sat(j+1, before(timefun[i] + span, timefun))
+  ensures  sat(i, eventuallynextwithin(x, span, timefun))
+{
+  TemporalAssist();
+}
 
-    lemma Lemma_EventuallyWithinSpansHelper(start:int, start':int, d:imap<int, int>, goal:temporal, span:int, timefun:imap<int, int>)
-        requires imaptotal(d);
-        requires imaptotal(timefun);
-        requires 1 <= span;
-        requires TLe(start, start');
-        requires forall i :: start <= i ==> 1 <= d[i];
-        requires sat(start, always(goalOrDecrease(goal, d, span, timefun)));
-        ensures  sat(start', eventuallywithin(goal, span * d[start'], timefun));
-        decreases d[start'];
+lemma Lemma_EventuallyWithinSpansHelper(start:int, start':int, d:imap<int, int>, goal:temporal, span:int, timefun:imap<int, int>)
+  requires imaptotal(d)
+  requires imaptotal(timefun)
+  requires 1 <= span
+  requires TLe(start, start')
+  requires forall i :: start <= i ==> 1 <= d[i]
+  requires sat(start, always(goalOrDecrease(goal, d, span, timefun)))
+  ensures  sat(start', eventuallywithin(goal, span * d[start'], timefun))
+  decreases d[start']
+{
+  TemporalAssist();
+  assert sat(start', goalOrDecrease(goal, d, span, timefun));
+  var n1 {:trigger TLe(start', n1)} :|
+         TLe(start', n1) && sat(n1, beforeabsolutetime(or(goal, stepDecrease(start', d)), timefun[start'] + span, timefun));
+  if (sat(n1, goal))
+  {
+    calc
     {
-        TemporalAssist();
-        assert sat(start', goalOrDecrease(goal, d, span, timefun));
-        var n1 {:trigger TLe(start', n1)} :|
-            TLe(start', n1) && sat(n1, beforeabsolutetime(or(goal, stepDecrease(start', d)), timefun[start'] + span, timefun));
-        if (sat(n1, goal))
+      1 <= d[start'];
+        { lemma_mul_inequality(1, d[start'], span); }
+      span * 1 <= span * d[start'];
+    }
+  }
+  else
+  {
+    Lemma_EventuallyWithinSpansHelper(start, n1, d, goal, span, timefun);
+    var n2 {:trigger TLe(n1, n2)} :|
+           TLe(n1, n2) && sat(n2, beforeabsolutetime(goal, timefun[n1] + span * d[n1], timefun));
+    calc
+    {
+      d[n1] + 1 <= d[start'];
+        { lemma_mul_inequality_forall(); lemma_mul_is_commutative_forall(); }
+      span * (d[n1] + 1) <= span * d[start'];
+        { lemma_mul_is_distributive_forall(); }
+      span * d[n1] + span <= span * d[start'];
+    }
+    assert sat(n2, beforeabsolutetime(goal, timefun[start'] + span * d[start'], timefun));
+  }
+}
+
+// If   []t :: <span>(goal || d < d[t])
+// and  [](0 <= d)
+// then []<span * d>(goal)
+lemma Lemma_EventuallyWithinSpans(start:int, d:imap<int, int>, goal:temporal, span:int, timefun:imap<int, int>)
+  requires imaptotal(d)
+  requires imaptotal(timefun)
+  requires 1 <= span
+  requires forall i :: start <= i ==> 1 <= d[i]
+  requires sat(start, always(goalOrDecrease(goal, d, span, timefun)))
+  ensures  sat(start, always(eventuallywithinspans(d, goal, span, timefun)))
+{
+  TemporalAssist();
+  forall start' | TLe(start, start')
+    ensures sat(start', eventuallywithin(goal, span * d[start'], timefun))
+  {
+    Lemma_EventuallyWithinSpansHelper(start, start', d, goal, span, timefun);
+  }
+}
+
+// If   []<span * d>(goal)
+// and  [](d <= n)
+// then []<span * n>(goal)
+lemma Lemma_EventuallyWithinBound(start:int, d:imap<int, int>, n:int, goal:temporal, span:int, timefun:imap<int, int>)
+  requires imaptotal(d)
+  requires imaptotal(timefun)
+  requires forall i :: d[i] <= n
+  requires 0 <= span
+  requires sat(start, always(eventuallywithinspans(d, goal, span, timefun)))
+  ensures  sat(start, always(eventuallywithin(goal, span * n, timefun)))
+{
+  TemporalAssist();
+  forall i1 | TLe(start, i1)
+    ensures sat(i1, eventuallywithin(goal, span * n, timefun))
+  {
+    lemma_mul_inequality_forall();
+    lemma_mul_is_commutative_forall();
+    assert span * d[i1] <= span * n;
+  }
+}
+
+lemma Lemma_EventuallynextWithinSpansHelper(start:int, start':int, d:imap<int, int>, goal:temporal, span:int, timefun:imap<int, int>)
+  requires imaptotal(d)
+  requires imaptotal(timefun)
+  requires 1 <= span
+  requires TLe(start, start')
+  requires forall i :: start <= i ==> 1 <= d[i]
+  requires sat(start, always(nextOrDecreaseWithin(goal, d, span, timefun)))
+  ensures  sat(start', eventuallynextwithin(goal, span * d[start'], timefun))
+  decreases d[start']
+{
+  TemporalAssist();
+  assert sat(start', nextOrDecreaseWithin(goal, d, span, timefun));
+  var n1 {:trigger TLe(start', n1)} :|
+         TLe(start', n1) && sat(n1, and(or(goal, nextDecrease(start', d)), next(before(timefun[start'] + span, timefun))));
+  if (sat(n1, goal))
+  {
+    calc
+    {
+      1 <= d[start'];
+        { lemma_mul_inequality(1, d[start'], span); }
+      span * 1 <= span * d[start'];
+    }
+  }
+  else
+  {
+    Lemma_EventuallynextWithinSpansHelper(start, n1 + 1, d, goal, span, timefun);
+    var n2 {:trigger TLe(n1 + 1, n2)} :| TLe(n1 + 1, n2)
+           && sat(n2, and(goal, next(before(timefun[n1 + 1] + span * d[n1 + 1], timefun))));
+    calc
+    {
+      d[n1 + 1] + 1 <= d[start'];
+        { lemma_mul_inequality_forall(); lemma_mul_is_commutative_forall(); }
+      span * (d[n1 + 1] + 1) <= span * d[start'];
+        { lemma_mul_is_distributive_forall(); }
+      span * d[n1 + 1] + span <= span * d[start'];
+    }
+    assert sat(n2, nextbefore(goal, timefun[start'] + span * d[start'], timefun));
+    assert sat(n2, and(goal, next(before(timefun[start'] + span * d[start'], timefun))));
+  }
+}
+
+// If   []t :: <span>(goal || d' < d[t]')
+// and  [](1 <= d)
+// then []<span * d>(goal)
+lemma Lemma_EventuallynextWithinSpans(start:int, d:imap<int, int>, goal:temporal, span:int, timefun:imap<int, int>)
+  requires imaptotal(d)
+  requires imaptotal(timefun)
+  requires 1 <= span
+  requires forall i :: start <= i ==> 1 <= d[i]
+  requires sat(start, always(nextOrDecreaseWithin(goal, d, span, timefun)))
+  ensures  sat(start, always(eventuallynextwithinspans(d, goal, span, timefun)))
+{
+  TemporalAssist();
+  forall start' | TLe(start, start')
+    ensures sat(start', eventuallynextwithin(goal, span * d[start'], timefun))
+  {
+    Lemma_EventuallynextWithinSpansHelper(start, start', d, goal, span, timefun);
+  }
+}
+
+// If   []<span * d>(goal)
+// and  [](d <= n)
+// then []<span * n>(goal)
+lemma Lemma_EventuallynextWithinBound(start:int, d:imap<int, int>, n:int, goal:temporal, span:int, timefun:imap<int, int>)
+  requires imaptotal(d)
+  requires imaptotal(timefun)
+  requires forall i :: d[i] <= n
+  requires 0 <= span
+  requires sat(start, always(eventuallynextwithinspans(d, goal, span, timefun)))
+  ensures  sat(start, always(eventuallynextwithin(goal, span * n, timefun)))
+{
+  TemporalAssist();
+  forall i1 | TLe(start, i1)
+    ensures sat(i1, eventuallynextwithin(goal, span * n, timefun))
+  {
+    lemma_mul_inequality_forall();
+    lemma_mul_is_commutative_forall();
+    assert span * d[i1] <= span * n;
+  }
+}
+
+lemma Lemma_EventuallynextWithinImpliesEventuallynext(i:int, x:temporal, span:int, timefun:imap<int, int>)
+  requires imaptotal(timefun)
+  requires sat(i, eventuallynextwithin(x, span, timefun))
+  ensures  sat(i, eventual(x))
+{
+  TemporalAssist();
+}
+
+lemma Lemma_AlwaysEventuallyWithinMeansAlwaysEventuallyWithinAfter(i:int, action:temporal, wait:int, span:int, timefun:imap<int, int>)
+  returns (step:int)
+  requires imaptotal(timefun)
+  requires monotonic_from(0, timefun)
+  requires wait >= 0
+  requires span >= 0
+  requires forall rt :: sat(0, eventual(after(rt, timefun)))
+  requires sat(i, always(eventuallynextwithin(action, span, timefun)))
+  requires 0 <= i
+  ensures  i <= step
+  ensures  sat(step, and(nextbefore(action, timefun[i] + wait + span, timefun), next(after(timefun[i] + wait, timefun))))
+  ensures  sat(i, eventual(and(nextbefore(action, timefun[i] + wait + span, timefun), next(after(timefun[i] + wait, timefun)))))
+{
+  var rt1 := timefun[i] + wait;
+  var rt2 := timefun[i] + wait + span;
+  var j := eventualStep(0, after(rt1, timefun));
+  Lemma_MonotonicFromImpliesMonotonicFromLater(0, i, timefun);
+  if (j < i)
+  {
+    j := i;
+  }
+  var k := stepattimeboundary(i, j, rt1, timefun);
+  TemporalDeduceFromAlways(i, k, eventuallynextwithin(action, span, timefun));
+  step := eventualStep(k, nextbefore(action, timefun[k] + span, timefun));
+  TemporalEventually(i, step, and(nextbefore(action, rt2, timefun), next(after(rt1, timefun))));
+}
+
+lemma Lemma_AlwaysEventuallyWithinImpliesAfter(i:int, j:int, action:temporal, span:int, timefun:imap<int, int>, rt:int) returns (step:int)
+  requires imaptotal(timefun)
+  requires monotonic_from(0, timefun)
+  requires span >= 0
+  requires forall t :: sat(0, eventual(after(t, timefun)))
+  requires sat(i, always(eventuallynextwithin(action, span, timefun)))
+  requires 0 <= i <= j
+  ensures  j <= step
+  ensures  sat(step, action)
+  ensures  rt <= timefun[step+1]
+{
+  assert sat(0, eventual(after(rt, timefun)));
+  var k := TemporalDeduceFromEventual(0, after(rt, timefun));
+  if k < j
+  {
+    assert rt <= timefun[k] <= timefun[j];
+    k := j;
+  }
+  TemporalDeduceFromAlways(i, k, eventuallynextwithin(action, span, timefun));
+  step := TemporalDeduceFromEventual(k, nextbefore(action, timefun[k] + span, timefun));
+}
+
+lemma Lemma_UntilAbsoluteTimeImpliesUntilEarlierTime(i:int, x:temporal, t1:int, t2:int, timefun:imap<int, int>)
+  requires imaptotal(timefun)
+  requires monotonic_from(i, timefun)
+  requires sat(i, untilabsolutetime(x, t1, timefun))
+  requires t2 <= t1
+  ensures  sat(i, untilabsolutetime(x, t2, timefun))
+{
+  TemporalAssist();
+}
+
+lemma Lemma_AlwaysUntilAbsoluteTimeImpliesAlwaysUntilEarlierTime(i:int, x:temporal, t1:int, t2:int, timefun:imap<int, int>)
+  requires imaptotal(timefun)
+  requires monotonic_from(i, timefun)
+  requires sat(i, always(untilabsolutetime(x, t1, timefun)))
+  requires t2 <= t1
+  ensures  sat(i, always(untilabsolutetime(x, t2, timefun)))
+{
+  TemporalAssist();
+}
+
+lemma TemporalDeduceFromEventuallyWithin(i:int, x:temporal, span:int, timefun:imap<int, int>) returns (step:int)
+  requires imaptotal(timefun)
+  requires sat(i, eventuallywithin(x, span, timefun))
+  ensures  i <= step
+  ensures  sat(step, beforeabsolutetime(x, timefun[i] + span, timefun))
+{
+  step := TemporalDeduceFromEventual(i, beforeabsolutetime(x, timefun[i] + span, timefun));
+}
+
+lemma TemporalDeduceFromEventuallyNextWithin(i:int, x:temporal, span:int, timefun:imap<int, int>) returns (step:int)
+  requires imaptotal(timefun)
+  requires sat(i, eventuallynextwithin(x, span, timefun))
+  ensures  i <= step
+  ensures  sat(step, nextbefore(x, timefun[i] + span, timefun))
+{
+  step := TemporalDeduceFromEventual(i, nextbefore(x, timefun[i] + span, timefun));
+}
+
+lemma TemporalDeduceFromAlwaysWithin(i:int, j:int, x:temporal, span:int, timefun:imap<int, int>)
+  requires imaptotal(timefun)
+  requires sat(i, alwayswithin(x, span, timefun))
+  requires i <= j
+  requires sat(j, before(timefun[i] + span, timefun))
+  ensures  sat(j, x)
+{
+  TemporalDeduceFromAlways(i, j, untilabsolutetime(x, timefun[i] + span, timefun));
+}
+
+predicate{:opaque} monotonic_from_opaque(start:int, f:imap<int, int>)
+{
+  forall i1, i2 :: i1 in f && i2 in f && start <= i1 <= i2 ==> f[i1] <= f[i2]
+}
+
+function{:opaque} actionGoalDecrease(i1:int, goal:temporal, d:imap<int, int>):temporal
+  requires imaptotal(d)
+  ensures  forall i {:trigger sat(i, actionGoalDecrease(i1, goal, d))} :: sat(i, actionGoalDecrease(i1, goal, d)) <==>
+               (0 < d[i + 1] && d[i + 1] < d[i1]) || sat(i, goal) || (d[i1] == 0)
+{
+  TemporalAssist();
+  stepmap(imap i :: (0 < d[i + 1] && d[i + 1] < d[i1]) || sat(i, goal) || (d[i1] == 0))
+}
+
+function{:opaque} actionGoalDecreaseWithin(goal:temporal, d:imap<int, int>, span:int, timefun:imap<int, int>):temporal
+  requires imaptotal(d)
+  requires imaptotal(timefun)
+  ensures  forall i {:trigger sat(i, actionGoalDecreaseWithin(goal, d, span, timefun))} ::
+               sat(i, actionGoalDecreaseWithin(goal, d, span, timefun)) <==>
+               sat(i, eventuallynextwithin(actionGoalDecrease(i, goal, d), span, timefun))
+{
+  TemporalAssist();
+  stepmap(imap i :: sat(i, eventuallynextwithin(actionGoalDecrease(i, goal, d), span, timefun)))
+}
+
+// If   []t :: <span>((0 < d' < d[t]') || goal || (d[t]' == 0))
+// and  [](0 <= d)
+// and  1 <= d
+// then <span * d>(goal)
+lemma Lemma_EventuallyNextGoalSpans(start:int, d:imap<int, int>, goal:temporal, span:int, timefun:imap<int, int>)
+  requires imaptotal(d)
+  requires imaptotal(timefun)
+  requires 1 <= span
+  requires 1 <= d[start]
+  requires forall i :: start <= i ==> 0 <= d[i]
+  requires sat(start, always(actionGoalDecreaseWithin(goal, d, span, timefun)))
+  ensures  sat(start, eventuallynextwithinspans(d, goal, span, timefun))
+  decreases d[start]
+{
+  TemporalAssist();
+  assert sat(start, actionGoalDecreaseWithin(goal, d, span, timefun));
+  var i1 {:trigger TLe(start, i1)} :|
+         TLe(start, i1) && sat(i1, actionGoalDecrease(start, goal, d)) && timefun[i1 + 1] <= timefun[start] + span;
+  if (sat(i1, goal))
+  {
+    calc
+    {
+      1 <= d[start];
+        { lemma_mul_inequality(1, d[start], span); }
+      span * 1 <= span * d[start];
+    }
+    assert sat(start, eventuallynextwithinspans(d, goal, span, timefun));
+  }
+  else
+  {
+    Lemma_EventuallyNextGoalSpans(i1 + 1, d, goal, span, timefun);
+    var i2 {:trigger TLe(i1 + 1, i2)} :| TLe(i1 + 1, i2)
+           && sat(i2, and(goal, next(before(timefun[i1 + 1] + span * d[i1 + 1], timefun))));
+    calc
+    {
+      d[i1 + 1] + 1 <= d[start];
+        { lemma_mul_inequality_forall(); lemma_mul_is_commutative_forall(); }
+      span * (d[i1 + 1] + 1) <= span * d[start];
+        { lemma_mul_is_distributive_forall(); }
+      span * d[i1 + 1] + span <= span * d[start];
+    }
+    assert sat(i2, nextbefore(goal, timefun[start] + span * d[start], timefun));
+    assert sat(i2, and(goal, next(before(timefun[start] + span * d[start], timefun))));
+  }
+}
+
+function {:opaque} ActionIsInstantaneousTemporal(x:temporal, timefun:imap<int, int>):temporal
+  requires imaptotal(timefun)
+  ensures  forall i {:trigger sat(i, ActionIsInstantaneousTemporal(x, timefun))} ::
+               sat(i, ActionIsInstantaneousTemporal(x, timefun)) <==> (sat(i, x) ==> timefun[i] == timefun[i+1])
+{
+  stepmap(imap i :: sat(i, x) ==> timefun[i] == timefun[i+1])
+}
+
+// "x" happens at most "count" times in all periods no longer than "span"
+function{:opaque} countWithinLe(count:int, x:temporal, span:int, timefun:imap<int, int>):temporal
+  requires imaptotal(timefun)
+  ensures  forall i1 {:trigger sat(i1, countWithinLe(count, x, span, timefun))} :: sat(i1, countWithinLe(count, x, span, timefun))
+                <==> (forall i2 :: TLe(i1, i2) && timefun[i2] <= timefun[i1] + span ==> countWithin(i1, i2, x) <= count)
+{
+  TemporalAssist();
+  stepmap(imap i1 :: forall i2 :: TLe(i1, i2) && timefun[i2] <= timefun[i1] + span ==> countWithin(i1, i2, x) <= count)
+}
+
+// "x" happens at least "count" times in a period no longer than "span"
+function{:opaque} countWithinGe(count:int, x:temporal, span:int, timefun:imap<int, int>):temporal
+  requires imaptotal(timefun)
+  ensures  forall i1 {:trigger sat(i1, countWithinGe(count, x, span, timefun))} :: sat(i1, countWithinGe(count, x, span, timefun))
+                <==> (exists i2 :: TLe(i1, i2) && timefun[i2] <= timefun[i1] + span && countWithin(i1, i2, x) >= count)
+{
+  TemporalAssist();
+  stepmap(imap i1 :: exists i2 :: TLe(i1, i2) && timefun[i2] <= timefun[i1] + span && countWithin(i1, i2, x) >= count)
+}
+
+lemma Lemma_CountWithinLeMultiple(start:int, n:nat, count:int, x:temporal, span:int, timefun:imap<int, int>)
+  requires imaptotal(timefun)
+  requires monotonic_from_opaque(start, timefun)
+  requires 1 <= n
+  requires 0 <= span
+  requires sat(start, always(ActionIsInstantaneousTemporal(x, timefun)))
+  requires sat(start, always(countWithinLe(count, x, span, timefun)))
+  ensures  sat(start, always(countWithinLe(count * n, x, span * n, timefun)))
+  decreases n
+{
+  TemporalAssist();
+  reveal_monotonic_from_opaque();
+  forall i1 | TLe(start, i1)
+    ensures sat(i1, countWithinLe(count * n, x, span * n, timefun))
+  {
+    if (n > 1)
+    {
+      forall i3 | TLe(i1, i3) && timefun[i3] <= timefun[i1] + span * n
+        ensures countWithin(i1, i3, x) <= count * n
+      {
+        Lemma_CountWithinLeMultiple(i1, n - 1, count, x, span, timefun);
+        assert sat(i1, countWithinLe(count * (n - 1), x, span * (n - 1), timefun));
+        assert forall i2 :: TLe(i1, i2) && timefun[i2] <= timefun[i1] + span * (n - 1) ==> countWithin(i1, i2, x) <= count * (n - 1);
+        if (exists i2' :: TLe(i1, i2') && TLe(i2', i3) && timefun[i2'] > timefun[i1] + span * (n - 1))
         {
-            calc
-            {
-                1 <= d[start'];
-                { lemma_mul_inequality(1, d[start'], span); }
-                span * 1 <= span * d[start'];
-            }
+          var f := imap i2' :: TLe(i2', i3) && timefun[i2'] > timefun[i1] + span * (n - 1);
+          var i2' := earliestStep(i1, stepmap(f));
+          lemma_mul_nonnegative(span, n-1);
+          var i2 := i2' - 1;
+          assert !sat(i2, stepmap(f));
+          TemporalDeduceFromAlways(i1, i2, ActionIsInstantaneousTemporal(x, timefun));
+          assert !sat(i2, x);
+          forall ensures 0 <= span * (n - 1) { lemma_mul_nonnegative(span, n - 1); }
+          assert TLe(i1, i2');
+          assert TLe(i1, i2);
+          assert TLe(i2, i3);
+          assert forall i :: i1 <= i <= i2 ==> !sat(i, stepmap(f));
+          assert forall i :: sat(i, stepmap(f)) == (TLe(i, i3) && timefun[i] > timefun[i1] + span * (n - 1));
+          assert forall i :: i1 <= i <= i2 ==> !(TLe(i, i3) && timefun[i] > timefun[i1] + span * (n - 1));
+          assert !(TLe(i2, i3) && timefun[i2] > timefun[i1] + span * (n - 1));
+          assert countWithin(i1, i2, x) <= count * (n - 1);
+
+          assert sat(i2', countWithinLe(count, x, span, timefun));
+          assert TLe(i2', i3) && timefun[i3] <= timefun[i2'] + span ==> countWithin(i2', i3, x) <= count;
+          forall
+            ensures span + span * (n - 1) == span * n
+            ensures count + count * (n - 1) == count * n
+          {
+            lemma_mul_auto();
+          }
+          assert countWithin(i2', i3, x) <= count;
+
+          assert actionsWithin(i1, i3, x) == actionsWithin(i1, i2, x) + actionsWithin(i2', i3, x);
+          assert |actionsWithin(i1, i3, x)| >= |actionsWithin(i1, i2, x)| + |actionsWithin(i2', i3, x)|;
         }
         else
         {
-            Lemma_EventuallyWithinSpansHelper(start, n1, d, goal, span, timefun);
-            var n2 {:trigger TLe(n1, n2)} :| TLe(n1, n2)
-                && sat(n2, beforeabsolutetime(goal, timefun[n1] + span * d[n1], timefun));
-            calc
-            {
-                d[n1] + 1 <= d[start'];
-                { lemma_mul_inequality_forall(); lemma_mul_is_commutative_forall(); }
-                span * (d[n1] + 1) <= span * d[start'];
-                { lemma_mul_is_distributive_forall(); }
-                span * d[n1] + span <= span * d[start'];
-            }
-            assert sat(n2, beforeabsolutetime(goal, timefun[start'] + span * d[start'], timefun));
+          assert forall i2' :: TLe(i1, i2') && TLe(i2', i3) ==> timefun[i2'] <= timefun[i1] + span * (n - 1);
+          assert timefun[i3] <= timefun[i1] + span * (n - 1);
+          assert countWithin(i1, i3, x) <= count * (n - 1);
+          forall ensures count * (n - 1) <= count * n { lemma_mul_auto(); }
         }
+      }
     }
+  }
+}
 
-    // If   []t :: <span>(goal || d < d[t])
-    // and  [](0 <= d)
-    // then []<span * d>(goal)
-    lemma Lemma_EventuallyWithinSpans(start:int, d:imap<int, int>, goal:temporal, span:int, timefun:imap<int, int>)
-        requires imaptotal(d);
-        requires imaptotal(timefun);
-        requires 1 <= span;
-        requires forall i :: start <= i ==> 1 <= d[i];
-        requires sat(start, always(goalOrDecrease(goal, d, span, timefun)));
-        ensures  sat(start, always(eventuallywithinspans(d, goal, span, timefun)));
+lemma Lemma_CountWithinGeMultiple(start:int, n:nat, count:int, x:temporal, span:int, timefun:imap<int, int>)
+  requires imaptotal(timefun)
+  requires monotonic_from_opaque(start, timefun)
+  requires 1 <= n
+  requires 0 <= span
+  requires sat(start, always(countWithinGe(count, x, span, timefun)))
+  ensures  sat(start, always(countWithinGe(count * n, x, span * n, timefun)))
+  decreases n
+{
+  TemporalAssist();
+  reveal_monotonic_from_opaque();
+  forall i1 | TLe(start, i1)
+    ensures sat(i1, countWithinGe(count * n, x, span * n, timefun))
+  {
+    if (n > 1)
     {
-        TemporalAssist();
-        forall start' | TLe(start, start')
-            ensures sat(start', eventuallywithin(goal, span * d[start'], timefun));
-        {
-            Lemma_EventuallyWithinSpansHelper(start, start', d, goal, span, timefun);
-        }
+      assert sat(i1, countWithinGe(count, x, span, timefun));
+      var i2 :| TLe(i1, i2) && timefun[i2] <= timefun[i1] + span && countWithin(i1, i2, x) >= count;
+      Lemma_CountWithinGeMultiple(i2, n - 1, count, x, span, timefun);
+      assert sat(i2, always(countWithinGe(count * (n - 1), x, span * (n - 1), timefun)));
+      assert sat(i2, countWithinGe(count * (n - 1), x, span * (n - 1), timefun));
+      var i3 :| TLe(i2, i3) && timefun[i3] <= timefun[i2] + span * (n - 1) && countWithin(i2, i3, x) >= count * (n - 1);
+      assert TLe(i1, i3);
+      assert actionsWithin(i1, i3, x) == actionsWithin(i1, i2, x) + actionsWithin(i2, i3, x);
+      assert |actionsWithin(i1, i3, x)| >= |actionsWithin(i1, i2, x)| + |actionsWithin(i2, i3, x)|;
+      forall
+        ensures span + span * (n - 1) == span * n
+        ensures count + count * (n - 1) == count * n
+      {
+        lemma_mul_auto();
+      }
     }
+  }
+}
 
-    // If   []<span * d>(goal)
-    // and  [](d <= n)
-    // then []<span * n>(goal)
-    lemma Lemma_EventuallyWithinBound(start:int, d:imap<int, int>, n:int, goal:temporal, span:int, timefun:imap<int, int>)
-        requires imaptotal(d);
-        requires imaptotal(timefun);
-        requires forall i :: d[i] <= n;
-        requires 0 <= span;
-        requires sat(start, always(eventuallywithinspans(d, goal, span, timefun)));
-        ensures  sat(start, always(eventuallywithin(goal, span * n, timefun)));
+lemma Lemma_CountWithinGeOne(start:int, x:temporal, span:int, timefun:imap<int, int>)
+  requires imaptotal(timefun)
+  requires 0 <= span
+  requires sat(start, always(eventuallynextwithin(x, span, timefun)))
+  ensures  sat(start, always(countWithinGe(1, x, span, timefun)))
+{
+  TemporalAssist();
+  forall i1 | TLe(start, i1)
+    ensures sat(i1, countWithinGe(1, x, span, timefun))
+  {
+    var i2 :| TLe(i1, i2) && sat(i2, nextbefore(x, timefun[i1] + span, timefun));
+    var i2' := i2 + 1;
+    assert i2 in actionsWithin(i1, i2', x);
+    assert countWithin(i1, i2', x) >= 1;
+  }
+}
+
+lemma{:timeLimitMultiplier 2} Lemma_CountIncrDecrHelper(i1:int, i2:int, d:imap<int, int>, nIncr:int, nDecr:int,
+  incr:temporal, decr:temporal)
+  requires imaptotal(d)
+  requires i1 <= i2
+  requires countWithin(i1, i2, decr) >= nDecr
+  requires countWithin(i1, i2, incr) <= nIncr
+  requires forall i {:trigger TLe(i1, i)}{:trigger sat(i, incr)}{:trigger sat(i, decr)} :: TLe(i1, i) && TLe(i, i2) ==>
+               || (sat(i, incr) && !sat(i, decr) && d[i + 1] == d[i] + 1)
+               || (!sat(i, incr) && sat(i, decr) && d[i + 1] < d[i])
+               || (!sat(i, incr) && !sat(i, decr) && d[i + 1] == d[i])
+  ensures  d[i2] <= d[i1] + nIncr - nDecr
+  decreases i2 - i1
+{
+  if (i1 == i2)
+  {
+    assert forall i :: i !in actionsWithin(i1, i2, decr);
+    assert actionsWithin(i1, i2, decr) == {};
+    assert countWithin(i1, i2, decr) == 0;
+  }
+  else
+  {
+    assert actionsWithin(i1, i2, incr) == actionsWithin(i1, i1 + 1, incr) + actionsWithin(i1 + 1, i2, incr);
+    assert actionsWithin(i1, i2, decr) == actionsWithin(i1, i1 + 1, decr) + actionsWithin(i1 + 1, i2, decr);
+    if (sat(i1, incr))
     {
-        TemporalAssist();
-        forall i1 | TLe(start, i1)
-            ensures sat(i1, eventuallywithin(goal, span * n, timefun));
-        {
-            lemma_mul_inequality_forall();
-            lemma_mul_is_commutative_forall();
-            assert span * d[i1] <= span * n;
-        }
+      assert i1 in actionsWithin(i1, i2, incr);
+      Lemma_CountIncrDecrHelper(i1 + 1, i2, d, nIncr - 1, nDecr, incr, decr);
     }
-
-    lemma Lemma_EventuallynextWithinSpansHelper(start:int, start':int, d:imap<int, int>, goal:temporal, span:int, timefun:imap<int, int>)
-        requires imaptotal(d);
-        requires imaptotal(timefun);
-        requires 1 <= span;
-        requires TLe(start, start');
-        requires forall i :: start <= i ==> 1 <= d[i];
-        requires sat(start, always(nextOrDecreaseWithin(goal, d, span, timefun)));
-        ensures  sat(start', eventuallynextwithin(goal, span * d[start'], timefun));
-        decreases d[start'];
+    else if (sat(i1, decr))
     {
-        TemporalAssist();
-        assert sat(start', nextOrDecreaseWithin(goal, d, span, timefun));
-        var n1 {:trigger TLe(start', n1)} :|
-            TLe(start', n1) && sat(n1, and(or(goal, nextDecrease(start', d)), next(before(timefun[start'] + span, timefun))));
-        if (sat(n1, goal))
-        {
-            calc
-            {
-                1 <= d[start'];
-                { lemma_mul_inequality(1, d[start'], span); }
-                span * 1 <= span * d[start'];
-            }
-        }
-        else
-        {
-            Lemma_EventuallynextWithinSpansHelper(start, n1 + 1, d, goal, span, timefun);
-            var n2 {:trigger TLe(n1 + 1, n2)} :| TLe(n1 + 1, n2)
-                && sat(n2, and(goal, next(before(timefun[n1 + 1] + span * d[n1 + 1], timefun))));
-            calc
-            {
-                d[n1 + 1] + 1 <= d[start'];
-                { lemma_mul_inequality_forall(); lemma_mul_is_commutative_forall(); }
-                span * (d[n1 + 1] + 1) <= span * d[start'];
-                { lemma_mul_is_distributive_forall(); }
-                span * d[n1 + 1] + span <= span * d[start'];
-            }
-            assert sat(n2, nextbefore(goal, timefun[start'] + span * d[start'], timefun));
-            assert sat(n2, and(goal, next(before(timefun[start'] + span * d[start'], timefun))));
-        }
+      forall j | i1 <= j < i1 + 1 && sat(j, decr)
+        ensures j == i1
+      {
+      }
+      assert i1 in actionsWithin(i1, i1 + 1, decr);
+      assert actionsWithin(i1, i1 + 1, decr) <= {i1};
+      assert actionsWithin(i1, i1 + 1, decr) == {i1};
+      Lemma_CountIncrDecrHelper(i1 + 1, i2, d, nIncr, nDecr - 1, incr, decr);
     }
-
-    // If   []t :: <span>(goal || d' < d[t]')
-    // and  [](1 <= d)
-    // then []<span * d>(goal)
-    lemma Lemma_EventuallynextWithinSpans(start:int, d:imap<int, int>, goal:temporal, span:int, timefun:imap<int, int>)
-        requires imaptotal(d);
-        requires imaptotal(timefun);
-        requires 1 <= span;
-        requires forall i :: start <= i ==> 1 <= d[i];
-        requires sat(start, always(nextOrDecreaseWithin(goal, d, span, timefun)));
-        ensures  sat(start, always(eventuallynextwithinspans(d, goal, span, timefun)));
+    else
     {
-        TemporalAssist();
-        forall start' | TLe(start, start')
-            ensures sat(start', eventuallynextwithin(goal, span * d[start'], timefun));
-        {
-            Lemma_EventuallynextWithinSpansHelper(start, start', d, goal, span, timefun);
-        }
+      Lemma_CountIncrDecrHelper(i1 + 1, i2, d, nIncr, nDecr, incr, decr);
     }
+  }
+}
 
-    // If   []<span * d>(goal)
-    // and  [](d <= n)
-    // then []<span * n>(goal)
-    lemma Lemma_EventuallynextWithinBound(start:int, d:imap<int, int>, n:int, goal:temporal, span:int, timefun:imap<int, int>)
-        requires imaptotal(d);
-        requires imaptotal(timefun);
-        requires forall i :: d[i] <= n;
-        requires 0 <= span;
-        requires sat(start, always(eventuallynextwithinspans(d, goal, span, timefun)));
-        ensures  sat(start, always(eventuallynextwithin(goal, span * n, timefun)));
+lemma Lemma_CountIncrDecr(i1:int, d:imap<int, int>, nIncr:int, nDecr:int, incr:temporal, decr:temporal, span:int, timefun:imap<int, int>)
+  returns (i2:int)
+  // |decr| >= nDecr
+  // |incr| <= nIncr
+  requires imaptotal(d)
+  requires imaptotal(timefun)
+  requires monotonic_from_opaque(i1, timefun)
+  requires 0 <= span
+  requires sat(i1, countWithinLe(nIncr, incr, span, timefun))
+  requires sat(i1, countWithinGe(nDecr, decr, span, timefun))
+  requires forall i {:trigger TLe(i1, i)} :: TLe(i1, i) && timefun[i] <= timefun[i1] + span ==>
+               || (sat(i, incr) && !sat(i, decr) && d[i + 1] == d[i] + 1)
+               || (!sat(i, incr) && sat(i, decr) && d[i + 1] < d[i])
+               || (!sat(i, incr) && !sat(i, decr) && d[i + 1] == d[i]);
+  ensures  timefun[i2] <= timefun[i1] + span
+  ensures  sat(i2, stepmap(imap i :: d[i] <= d[i1] + nIncr - nDecr))
+  ensures  sat(i1, alwayswithin(stepmap(imap i :: d[i] <= d[i1] + nIncr), span, timefun))
+  ensures  nDecr > 0 ==> i2 > i1
+{
+  TemporalAssist();
+  reveal_monotonic_from_opaque();
+  i2 :| TLe(i1, i2) && timefun[i2] <= timefun[i1] + span && countWithin(i1, i2, decr) >= nDecr;
+  assert TLe(i1, i2) && timefun[i2] <= timefun[i1] + span ==> countWithin(i1, i2, incr) <= nIncr;
+
+  assert countWithin(i1, i2, decr) >= nDecr;
+  assert countWithin(i1, i2, incr) <= nIncr;
+  Lemma_CountIncrDecrHelper(i1, i2, d, nIncr, nDecr, incr, decr);
+  assert d[i2] <= d[i1] + nIncr - nDecr;
+
+  var f1 := imap i :: d[i] <= d[i1] + nIncr - nDecr;
+  assert sat(i2, stepmap(f1));
+  assert sat(i1, eventuallywithin(stepmap(f1), span, timefun));
+
+  var f2 := imap i :: d[i] <= d[i1] + nIncr;
+  forall i | TLe(i1, i) && timefun[i] <= timefun[i1] + span
+    ensures f2[i]
+  {
+    Lemma_CountIncrDecrHelper(i1, i, d, nIncr, countWithin(i1, i, decr), incr, decr);
+    assert d[i] <= d[i1] + nIncr;
+  }
+  assert sat(i1, alwayswithin(stepmap(f2), span, timefun));
+}
+
+lemma Lemma_CountIncrHelper(i1:int, i2:int, d:imap<int, int>, nIncr:int, incr:temporal)
+  requires imaptotal(d)
+  requires i1 <= i2
+  requires countWithin(i1, i2, incr) <= nIncr
+  requires forall i {:trigger TLe(i1, i)}{:trigger sat(i, incr)} :: TLe(i1, i) && TLe(i, i2) ==>
+               || (sat(i, incr) && d[i + 1] == d[i] + 1)
+               || (!sat(i, incr) && d[i + 1] <= d[i])
+  ensures  d[i2] <= d[i1] + nIncr
+  decreases i2 - i1
+{
+  if (i1 != i2)
+  {
+    assert actionsWithin(i1, i2, incr) == actionsWithin(i1, i1 + 1, incr) + actionsWithin(i1 + 1, i2, incr);
+    if (sat(i1, incr))
     {
-        TemporalAssist();
-        forall i1 | TLe(start, i1)
-            ensures sat(i1, eventuallynextwithin(goal, span * n, timefun));
-        {
-            lemma_mul_inequality_forall();
-            lemma_mul_is_commutative_forall();
-            assert span * d[i1] <= span * n;
-        }
+      assert i1 in actionsWithin(i1, i2, incr);
+      Lemma_CountIncrHelper(i1 + 1, i2, d, nIncr - 1, incr);
     }
-
-    lemma Lemma_EventuallynextWithinImpliesEventuallynext(i:int, x:temporal, span:int, timefun:imap<int, int>)
-        requires imaptotal(timefun);
-        requires sat(i, eventuallynextwithin(x, span, timefun));
-        ensures  sat(i, eventual(x));
+    else
     {
-        TemporalAssist();
+      Lemma_CountIncrHelper(i1 + 1, i2, d, nIncr, incr);
     }
+  }
+}
 
-    lemma Lemma_AlwaysEventuallyWithinMeansAlwaysEventuallyWithinAfter(i:int, action:temporal, wait:int, span:int, timefun:imap<int, int>) returns (step:int)
-        requires imaptotal(timefun);
-        requires monotonic_from(0, timefun);
-        requires wait >= 0;
-        requires span >= 0;
-        requires forall rt :: sat(0, eventual(after(rt, timefun)));
-        requires sat(i, always(eventuallynextwithin(action, span, timefun)));
-        requires 0 <= i;
-        ensures  i <= step;
-        ensures  sat(step, and(nextbefore(action, timefun[i] + wait + span, timefun),
-                               next(after(timefun[i] + wait, timefun))));
-        ensures  sat(i, eventual(and(nextbefore(action, timefun[i] + wait + span, timefun),
-                                     next(after(timefun[i] + wait, timefun)))));
-    {
-        var rt1 := timefun[i] + wait;
-        var rt2 := timefun[i] + wait + span;
-        var j := eventualStep(0, after(rt1, timefun));
-        Lemma_MonotonicFromImpliesMonotonicFromLater(0, i, timefun);
-        if (j < i)
-        {
-            j := i;
-        }
-        var k := stepattimeboundary(i, j, rt1, timefun);
-        TemporalDeduceFromAlways(i, k, eventuallynextwithin(action, span, timefun));
-        step := eventualStep(k, nextbefore(action, timefun[k] + span, timefun));
-        TemporalEventually(i, step, and(nextbefore(action, rt2, timefun),
-                                        next(after(rt1, timefun))));
-    }
+lemma Lemma_CountIncr(i1:int, d:imap<int, int>, nIncr:int, incr:temporal, span:int, timefun:imap<int, int>)
+  // |incr| <= nIncr
+  requires imaptotal(d)
+  requires imaptotal(timefun)
+  requires monotonic_from_opaque(i1, timefun)
+  requires 0 <= span
+  requires sat(i1, countWithinLe(nIncr, incr, span, timefun))
+  requires forall i {:trigger TLe(i1, i)} :: TLe(i1, i) && timefun[i] <= timefun[i1] + span ==>
+               || (sat(i, incr) && d[i + 1] == d[i] + 1)
+               || (!sat(i, incr) && d[i + 1] <= d[i])
+  ensures  sat(i1, alwayswithin(stepmap(imap i :: d[i] <= d[i1] + nIncr), span, timefun))
+{
+  TemporalAssist();
+  reveal_monotonic_from_opaque();
 
-    lemma Lemma_AlwaysEventuallyWithinImpliesAfter(i:int, j:int, action:temporal, span:int, timefun:imap<int, int>, rt:int) returns (step:int)
-        requires imaptotal(timefun);
-        requires monotonic_from(0, timefun);
-        requires span >= 0;
-        requires forall t :: sat(0, eventual(after(t, timefun)));
-        requires sat(i, always(eventuallynextwithin(action, span, timefun)));
-        requires 0 <= i <= j;
-        ensures  j <= step;
-        ensures  sat(step, action);
-        ensures  rt <= timefun[step+1];
-    {
-        assert sat(0, eventual(after(rt, timefun)));
-        var k := TemporalDeduceFromEventual(0, after(rt, timefun));
-        if k < j
-        {
-            assert rt <= timefun[k] <= timefun[j];
-            k := j;
-        }
-        TemporalDeduceFromAlways(i, k, eventuallynextwithin(action, span, timefun));
-        step := TemporalDeduceFromEventual(k, nextbefore(action, timefun[k] + span, timefun));
-    }
-
-    lemma Lemma_UntilAbsoluteTimeImpliesUntilEarlierTime(i:int, x:temporal, t1:int, t2:int, timefun:imap<int, int>)
-        requires imaptotal(timefun);
-        requires monotonic_from(i, timefun);
-        requires sat(i, untilabsolutetime(x, t1, timefun));
-        requires t2 <= t1;
-        ensures  sat(i, untilabsolutetime(x, t2, timefun));
-    {
-        TemporalAssist();
-    }
-
-    lemma Lemma_AlwaysUntilAbsoluteTimeImpliesAlwaysUntilEarlierTime(i:int, x:temporal, t1:int, t2:int, timefun:imap<int, int>)
-        requires imaptotal(timefun);
-        requires monotonic_from(i, timefun);
-        requires sat(i, always(untilabsolutetime(x, t1, timefun)));
-        requires t2 <= t1;
-        ensures  sat(i, always(untilabsolutetime(x, t2, timefun)));
-    {
-        TemporalAssist();
-    }
-
-    lemma TemporalDeduceFromEventuallyWithin(i:int, x:temporal, span:int, timefun:imap<int, int>) returns (step:int)
-        requires imaptotal(timefun);
-        requires sat(i, eventuallywithin(x, span, timefun));
-        ensures  i <= step;
-        ensures  sat(step, beforeabsolutetime(x, timefun[i] + span, timefun));
-    {
-        step := TemporalDeduceFromEventual(i, beforeabsolutetime(x, timefun[i] + span, timefun));
-    }
-
-    lemma TemporalDeduceFromEventuallyNextWithin(i:int, x:temporal, span:int, timefun:imap<int, int>) returns (step:int)
-        requires imaptotal(timefun);
-        requires sat(i, eventuallynextwithin(x, span, timefun));
-        ensures  i <= step;
-        ensures  sat(step, nextbefore(x, timefun[i] + span, timefun));
-    {
-        step := TemporalDeduceFromEventual(i, nextbefore(x, timefun[i] + span, timefun));
-    }
-
-    lemma TemporalDeduceFromAlwaysWithin(i:int, j:int, x:temporal, span:int, timefun:imap<int, int>)
-        requires imaptotal(timefun);
-        requires sat(i, alwayswithin(x, span, timefun));
-        requires i <= j;
-        requires sat(j, before(timefun[i] + span, timefun));
-        ensures  sat(j, x);
-    {
-        TemporalDeduceFromAlways(i, j, untilabsolutetime(x, timefun[i] + span, timefun));
-    }
-
-    predicate{:opaque} monotonic_from_opaque(start:int, f:imap<int, int>)
-    {
-        forall i1, i2 :: i1 in f && i2 in f && start <= i1 <= i2 ==> f[i1] <= f[i2]
-    }
-
-    function{:opaque} actionGoalDecrease(i1:int, goal:temporal, d:imap<int, int>):temporal
-        requires imaptotal(d);
-        ensures  forall i {:trigger sat(i, actionGoalDecrease(i1, goal, d))} :: sat(i, actionGoalDecrease(i1, goal, d)) <==>
-                    (0 < d[i + 1] && d[i + 1] < d[i1]) || sat(i, goal) || (d[i1] == 0);
-    {
-        TemporalAssist();
-        stepmap(imap i :: (0 < d[i + 1] && d[i + 1] < d[i1]) || sat(i, goal) || (d[i1] == 0))
-    }
-
-    function{:opaque} actionGoalDecreaseWithin(goal:temporal, d:imap<int, int>, span:int, timefun:imap<int, int>):temporal
-        requires imaptotal(d);
-        requires imaptotal(timefun);
-        ensures  forall i {:trigger sat(i, actionGoalDecreaseWithin(goal, d, span, timefun))} :: sat(i, actionGoalDecreaseWithin(goal, d, span, timefun)) <==>
-                    sat(i, eventuallynextwithin(actionGoalDecrease(i, goal, d), span, timefun));
-    {
-        TemporalAssist();
-        stepmap(imap i :: sat(i, eventuallynextwithin(actionGoalDecrease(i, goal, d), span, timefun)))
-    }
-
-    // If   []t :: <span>((0 < d' < d[t]') || goal || (d[t]' == 0))
-    // and  [](0 <= d)
-    // and  1 <= d
-    // then <span * d>(goal)
-    lemma Lemma_EventuallyNextGoalSpans(start:int, d:imap<int, int>, goal:temporal, span:int, timefun:imap<int, int>)
-        requires imaptotal(d);
-        requires imaptotal(timefun);
-        requires 1 <= span;
-        requires 1 <= d[start];
-        requires forall i :: start <= i ==> 0 <= d[i];
-        requires sat(start, always(actionGoalDecreaseWithin(goal, d, span, timefun)));
-        ensures  sat(start, eventuallynextwithinspans(d, goal, span, timefun));
-        decreases d[start];
-    {
-        TemporalAssist();
-        assert sat(start, actionGoalDecreaseWithin(goal, d, span, timefun));
-        var i1 {:trigger TLe(start, i1)} :|
-            TLe(start, i1) && sat(i1, actionGoalDecrease(start, goal, d)) && timefun[i1 + 1] <= timefun[start] + span;
-        if (sat(i1, goal))
-        {
-            calc
-            {
-                1 <= d[start];
-                { lemma_mul_inequality(1, d[start], span); }
-                span * 1 <= span * d[start];
-            }
-            assert sat(start, eventuallynextwithinspans(d, goal, span, timefun));
-        }
-        else
-        {
-            Lemma_EventuallyNextGoalSpans(i1 + 1, d, goal, span, timefun);
-            var i2 {:trigger TLe(i1 + 1, i2)} :| TLe(i1 + 1, i2)
-                && sat(i2, and(goal, next(before(timefun[i1 + 1] + span * d[i1 + 1], timefun))));
-            calc
-            {
-                d[i1 + 1] + 1 <= d[start];
-                { lemma_mul_inequality_forall(); lemma_mul_is_commutative_forall(); }
-                span * (d[i1 + 1] + 1) <= span * d[start];
-                { lemma_mul_is_distributive_forall(); }
-                span * d[i1 + 1] + span <= span * d[start];
-            }
-            assert sat(i2, nextbefore(goal, timefun[start] + span * d[start], timefun));
-            assert sat(i2, and(goal, next(before(timefun[start] + span * d[start], timefun))));
-        }
-    }
-
-    function {:opaque} ActionIsInstantaneousTemporal(x:temporal, timefun:imap<int, int>):temporal
-        requires imaptotal(timefun);
-        ensures  forall i {:trigger sat(i, ActionIsInstantaneousTemporal(x, timefun))} ::
-                 sat(i, ActionIsInstantaneousTemporal(x, timefun)) <==> (sat(i, x) ==> timefun[i] == timefun[i+1]);
-    {
-        stepmap(imap i :: sat(i, x) ==> timefun[i] == timefun[i+1])
-    }
-
-    // "x" happens at most "count" times in all periods no longer than "span"
-    function{:opaque} countWithinLe(count:int, x:temporal, span:int, timefun:imap<int, int>):temporal
-        requires imaptotal(timefun);
-        ensures  forall i1 {:trigger sat(i1, countWithinLe(count, x, span, timefun))} :: sat(i1, countWithinLe(count, x, span, timefun))
-                    <==> (forall i2 :: TLe(i1, i2) && timefun[i2] <= timefun[i1] + span ==> countWithin(i1, i2, x) <= count);
-    {
-        TemporalAssist();
-        stepmap(imap i1 :: forall i2 :: TLe(i1, i2) && timefun[i2] <= timefun[i1] + span ==> countWithin(i1, i2, x) <= count)
-    }
-
-    // "x" happens at least "count" times in a period no longer than "span"
-    function{:opaque} countWithinGe(count:int, x:temporal, span:int, timefun:imap<int, int>):temporal
-        requires imaptotal(timefun);
-        ensures  forall i1 {:trigger sat(i1, countWithinGe(count, x, span, timefun))} :: sat(i1, countWithinGe(count, x, span, timefun))
-                    <==> (exists i2 :: TLe(i1, i2) && timefun[i2] <= timefun[i1] + span && countWithin(i1, i2, x) >= count);
-    {
-        TemporalAssist();
-        stepmap(imap i1 :: exists i2 :: TLe(i1, i2) && timefun[i2] <= timefun[i1] + span && countWithin(i1, i2, x) >= count)
-    }
-
-    lemma Lemma_CountWithinLeMultiple(start:int, n:nat, count:int, x:temporal, span:int, timefun:imap<int, int>)
-        requires imaptotal(timefun);
-        requires monotonic_from_opaque(start, timefun);
-        requires 1 <= n;
-        requires 0 <= span;
-        requires sat(start, always(ActionIsInstantaneousTemporal(x, timefun)));
-        requires sat(start, always(countWithinLe(count, x, span, timefun)));
-        ensures  sat(start, always(countWithinLe(count * n, x, span * n, timefun)));
-        decreases n;
-    {
-        TemporalAssist();
-        reveal_monotonic_from_opaque();
-        forall i1 | TLe(start, i1)
-            ensures sat(i1, countWithinLe(count * n, x, span * n, timefun));
-        {
-            if (n > 1)
-            {
-                forall i3 | TLe(i1, i3) && timefun[i3] <= timefun[i1] + span * n
-                    ensures countWithin(i1, i3, x) <= count * n;
-                {
-                    Lemma_CountWithinLeMultiple(i1, n - 1, count, x, span, timefun);
-                    assert sat(i1, countWithinLe(count * (n - 1), x, span * (n - 1), timefun));
-                    assert forall i2 :: TLe(i1, i2) && timefun[i2] <= timefun[i1] + span * (n - 1) ==> countWithin(i1, i2, x) <= count * (n - 1);
-                    if (exists i2' :: TLe(i1, i2') && TLe(i2', i3) && timefun[i2'] > timefun[i1] + span * (n - 1))
-                    {
-                        var f := imap i2' :: TLe(i2', i3) && timefun[i2'] > timefun[i1] + span * (n - 1);
-                        var i2' := earliestStep(i1, stepmap(f));
-                        lemma_mul_nonnegative(span, n-1);
-                        var i2 := i2' - 1;
-                        assert !sat(i2, stepmap(f));
-                        TemporalDeduceFromAlways(i1, i2, ActionIsInstantaneousTemporal(x, timefun));
-                        assert !sat(i2, x);
-                        forall ensures 0 <= span * (n - 1) { lemma_mul_nonnegative(span, n - 1); }
-                        assert TLe(i1, i2');
-                        assert TLe(i1, i2);
-                        assert TLe(i2, i3);
-                        assert forall i :: i1 <= i <= i2 ==> !sat(i, stepmap(f));
-                        assert forall i :: sat(i, stepmap(f)) == (TLe(i, i3) && timefun[i] > timefun[i1] + span * (n - 1));
-                        assert forall i :: i1 <= i <= i2 ==> !(TLe(i, i3) && timefun[i] > timefun[i1] + span * (n - 1));
-                        assert !(TLe(i2, i3) && timefun[i2] > timefun[i1] + span * (n - 1));
-                        assert countWithin(i1, i2, x) <= count * (n - 1);
-
-                        assert sat(i2', countWithinLe(count, x, span, timefun));
-                        assert TLe(i2', i3) && timefun[i3] <= timefun[i2'] + span ==> countWithin(i2', i3, x) <= count;
-                        forall
-                            ensures span + span * (n - 1) == span * n;
-                            ensures count + count * (n - 1) == count * n;
-                        {
-                            lemma_mul_auto();
-                        }
-                        assert countWithin(i2', i3, x) <= count;
-
-                        assert actionsWithin(i1, i3, x) == actionsWithin(i1, i2, x) + actionsWithin(i2', i3, x);
-                        assert |actionsWithin(i1, i3, x)| >= |actionsWithin(i1, i2, x)| + |actionsWithin(i2', i3, x)|;
-                    }
-                    else
-                    {
-                        assert forall i2' :: TLe(i1, i2') && TLe(i2', i3) ==> timefun[i2'] <= timefun[i1] + span * (n - 1);
-                        assert timefun[i3] <= timefun[i1] + span * (n - 1);
-                        assert countWithin(i1, i3, x) <= count * (n - 1);
-                        forall ensures count * (n - 1) <= count * n; { lemma_mul_auto(); }
-                    }
-                }
-            }
-        }
-    }
-
-    lemma Lemma_CountWithinGeMultiple(start:int, n:nat, count:int, x:temporal, span:int, timefun:imap<int, int>)
-        requires imaptotal(timefun);
-        requires monotonic_from_opaque(start, timefun);
-        requires 1 <= n;
-        requires 0 <= span;
-        requires sat(start, always(countWithinGe(count, x, span, timefun)));
-        ensures  sat(start, always(countWithinGe(count * n, x, span * n, timefun)));
-        decreases n;
-    {
-        TemporalAssist();
-        reveal_monotonic_from_opaque();
-        forall i1 | TLe(start, i1)
-            ensures sat(i1, countWithinGe(count * n, x, span * n, timefun));
-        {
-            if (n > 1)
-            {
-                assert sat(i1, countWithinGe(count, x, span, timefun));
-                var i2 :| TLe(i1, i2) && timefun[i2] <= timefun[i1] + span && countWithin(i1, i2, x) >= count;
-                Lemma_CountWithinGeMultiple(i2, n - 1, count, x, span, timefun);
-                assert sat(i2, always(countWithinGe(count * (n - 1), x, span * (n - 1), timefun)));
-                assert sat(i2, countWithinGe(count * (n - 1), x, span * (n - 1), timefun));
-                var i3 :| TLe(i2, i3) && timefun[i3] <= timefun[i2] + span * (n - 1) && countWithin(i2, i3, x) >= count * (n - 1);
-                assert TLe(i1, i3);
-                assert actionsWithin(i1, i3, x) == actionsWithin(i1, i2, x) + actionsWithin(i2, i3, x);
-                assert |actionsWithin(i1, i3, x)| >= |actionsWithin(i1, i2, x)| + |actionsWithin(i2, i3, x)|;
-                forall
-                    ensures span + span * (n - 1) == span * n;
-                    ensures count + count * (n - 1) == count * n;
-                {
-                    lemma_mul_auto();
-                }
-            }
-        }
-    }
-
-    lemma Lemma_CountWithinGeOne(start:int, x:temporal, span:int, timefun:imap<int, int>)
-        requires imaptotal(timefun);
-        requires 0 <= span;
-        requires sat(start, always(eventuallynextwithin(x, span, timefun)));
-        ensures  sat(start, always(countWithinGe(1, x, span, timefun)));
-    {
-        TemporalAssist();
-        forall i1 | TLe(start, i1)
-            ensures sat(i1, countWithinGe(1, x, span, timefun));
-        {
-            var i2 :| TLe(i1, i2) && sat(i2, nextbefore(x, timefun[i1] + span, timefun));
-            var i2' := i2 + 1;
-            assert i2 in actionsWithin(i1, i2', x);
-            assert countWithin(i1, i2', x) >= 1;
-        }
-    }
-
-    lemma{:timeLimitMultiplier 2} Lemma_CountIncrDecrHelper(i1:int, i2:int, d:imap<int, int>, nIncr:int, nDecr:int, incr:temporal, decr:temporal)
-        requires imaptotal(d);
-        requires i1 <= i2;
-        requires countWithin(i1, i2, decr) >= nDecr;
-        requires countWithin(i1, i2, incr) <= nIncr;
-        requires forall i {:trigger TLe(i1, i)}{:trigger sat(i, incr)}{:trigger sat(i, decr)} :: TLe(i1, i) && TLe(i, i2) ==>
-                        (sat(i, incr) && !sat(i, decr) && d[i + 1] == d[i] + 1)
-                     || (!sat(i, incr) && sat(i, decr) && d[i + 1] < d[i])
-                     || (!sat(i, incr) && !sat(i, decr) && d[i + 1] == d[i]);
-        ensures  d[i2] <= d[i1] + nIncr - nDecr;
-        decreases i2 - i1;
-    {
-        if (i1 == i2)
-        {
-            assert forall i :: i !in actionsWithin(i1, i2, decr);
-            assert actionsWithin(i1, i2, decr) == {};
-            assert countWithin(i1, i2, decr) == 0;
-        }
-        else
-        {
-            assert actionsWithin(i1, i2, incr) == actionsWithin(i1, i1 + 1, incr) + actionsWithin(i1 + 1, i2, incr);
-            assert actionsWithin(i1, i2, decr) == actionsWithin(i1, i1 + 1, decr) + actionsWithin(i1 + 1, i2, decr);
-            if (sat(i1, incr))
-            {
-                assert i1 in actionsWithin(i1, i2, incr);
-                Lemma_CountIncrDecrHelper(i1 + 1, i2, d, nIncr - 1, nDecr, incr, decr);
-            }
-            else if (sat(i1, decr))
-            {
-                forall j | i1 <= j < i1 + 1 && sat(j, decr)
-                    ensures j == i1;
-                {
-                }
-                assert i1 in actionsWithin(i1, i1 + 1, decr);
-                assert actionsWithin(i1, i1 + 1, decr) <= {i1};
-                assert actionsWithin(i1, i1 + 1, decr) == {i1};
-                Lemma_CountIncrDecrHelper(i1 + 1, i2, d, nIncr, nDecr - 1, incr, decr);
-            }
-            else
-            {
-                Lemma_CountIncrDecrHelper(i1 + 1, i2, d, nIncr, nDecr, incr, decr);
-            }
-        }
-    }
-
-    lemma Lemma_CountIncrDecr(i1:int, d:imap<int, int>, nIncr:int, nDecr:int, incr:temporal, decr:temporal, span:int, timefun:imap<int, int>)
-        returns (i2:int)
-        // |decr| >= nDecr
-        // |incr| <= nIncr
-        requires imaptotal(d);
-        requires imaptotal(timefun);
-        requires monotonic_from_opaque(i1, timefun);
-        requires 0 <= span;
-        requires sat(i1, countWithinLe(nIncr, incr, span, timefun));
-        requires sat(i1, countWithinGe(nDecr, decr, span, timefun));
-        requires forall i {:trigger TLe(i1, i)} :: TLe(i1, i) && timefun[i] <= timefun[i1] + span ==>
-                        (sat(i, incr) && !sat(i, decr) && d[i + 1] == d[i] + 1)
-                     || (!sat(i, incr) && sat(i, decr) && d[i + 1] < d[i])
-                     || (!sat(i, incr) && !sat(i, decr) && d[i + 1] == d[i]);
-        ensures  timefun[i2] <= timefun[i1] + span;
-        ensures  sat(i2, stepmap(imap i :: d[i] <= d[i1] + nIncr - nDecr));
-        ensures  sat(i1, alwayswithin(stepmap(imap i :: d[i] <= d[i1] + nIncr), span, timefun));
-        ensures  nDecr > 0 ==> i2 > i1;
-    {
-        TemporalAssist();
-        reveal_monotonic_from_opaque();
-        i2 :| TLe(i1, i2) && timefun[i2] <= timefun[i1] + span && countWithin(i1, i2, decr) >= nDecr;
-        assert TLe(i1, i2) && timefun[i2] <= timefun[i1] + span ==> countWithin(i1, i2, incr) <= nIncr;
-
-        assert countWithin(i1, i2, decr) >= nDecr;
-        assert countWithin(i1, i2, incr) <= nIncr;
-        Lemma_CountIncrDecrHelper(i1, i2, d, nIncr, nDecr, incr, decr);
-        assert d[i2] <= d[i1] + nIncr - nDecr;
-
-        var f1 := imap i :: d[i] <= d[i1] + nIncr - nDecr;
-        assert sat(i2, stepmap(f1));
-        assert sat(i1, eventuallywithin(stepmap(f1), span, timefun));
-
-        var f2 := imap i :: d[i] <= d[i1] + nIncr;
-        forall i | TLe(i1, i) && timefun[i] <= timefun[i1] + span
-            ensures f2[i];
-        {
-            Lemma_CountIncrDecrHelper(i1, i, d, nIncr, countWithin(i1, i, decr), incr, decr);
-            assert d[i] <= d[i1] + nIncr;
-        }
-        assert sat(i1, alwayswithin(stepmap(f2), span, timefun));
-    }
-
-    lemma Lemma_CountIncrHelper(i1:int, i2:int, d:imap<int, int>, nIncr:int, incr:temporal)
-        requires imaptotal(d);
-        requires i1 <= i2;
-        requires countWithin(i1, i2, incr) <= nIncr;
-        requires forall i {:trigger TLe(i1, i)}{:trigger sat(i, incr)} :: TLe(i1, i) && TLe(i, i2) ==>
-                        (sat(i, incr) && d[i + 1] == d[i] + 1)
-                     || (!sat(i, incr) && d[i + 1] <= d[i])
-        ensures  d[i2] <= d[i1] + nIncr;
-        decreases i2 - i1;
-    {
-        if (i1 != i2)
-        {
-            assert actionsWithin(i1, i2, incr) == actionsWithin(i1, i1 + 1, incr) + actionsWithin(i1 + 1, i2, incr);
-            if (sat(i1, incr))
-            {
-                assert i1 in actionsWithin(i1, i2, incr);
-                Lemma_CountIncrHelper(i1 + 1, i2, d, nIncr - 1, incr);
-            }
-            else
-            {
-                Lemma_CountIncrHelper(i1 + 1, i2, d, nIncr, incr);
-            }
-        }
-    }
-
-    lemma Lemma_CountIncr(i1:int, d:imap<int, int>, nIncr:int, incr:temporal, span:int, timefun:imap<int, int>)
-        // |incr| <= nIncr
-        requires imaptotal(d);
-        requires imaptotal(timefun);
-        requires monotonic_from_opaque(i1, timefun);
-        requires 0 <= span;
-        requires sat(i1, countWithinLe(nIncr, incr, span, timefun));
-        requires forall i {:trigger TLe(i1, i)} :: TLe(i1, i) && timefun[i] <= timefun[i1] + span ==>
-                        (sat(i, incr) && d[i + 1] == d[i] + 1)
-                     || (!sat(i, incr) && d[i + 1] <= d[i])
-        ensures  sat(i1, alwayswithin(stepmap(imap i :: d[i] <= d[i1] + nIncr), span, timefun));
-    {
-        TemporalAssist();
-        reveal_monotonic_from_opaque();
-
-        var f2 := imap i :: d[i] <= d[i1] + nIncr;
-        forall i | TLe(i1, i) && timefun[i] <= timefun[i1] + span
-            ensures f2[i];
-        {
-            Lemma_CountIncrHelper(i1, i, d, nIncr, incr);
-            assert d[i] <= d[i1] + nIncr;
-        }
-        assert sat(i1, alwayswithin(stepmap(f2), span, timefun));
-    }
+  var f2 := imap i :: d[i] <= d[i1] + nIncr;
+  forall i | TLe(i1, i) && timefun[i] <= timefun[i1] + span
+    ensures f2[i]
+  {
+    Lemma_CountIncrHelper(i1, i, d, nIncr, incr);
+    assert d[i] <= d[i1] + nIncr;
+  }
+  assert sat(i1, alwayswithin(stepmap(f2), span, timefun));
+}
 
 } 
