ironfleet/src/Dafny/Libraries/Math/div_nonlinear.i.dfy
@@ -11,53 +11,53 @@ module Math__div_nonlinear_i {
 // it in div.i.dfy using the connection to the recursive definition
 
 lemma lemma_div_of_0(d:int)
-    requires d != 0;
-    ensures 0/d == 0;
+  requires d != 0
+  ensures 0/d == 0
 { }
 
 lemma lemma_div_by_self(d:int)
-    requires d != 0;
-    ensures d/d == 1;
+  requires d != 0
+  ensures d/d == 1
 { }
 
 lemma lemma_small_div()
-    ensures forall x, d {:trigger x / d} :: 0 <= x < d && d > 0 ==> x / d == 0;
+  ensures forall x, d {:trigger x / d} :: 0 <= x < d && d > 0 ==> x / d == 0
 { }
 
 lemma lemma_mod_of_zero_is_zero(m:int)
-    requires 0 < m;
-    ensures 0 % m == 0;
+  requires 0 < m
+  ensures 0 % m == 0
 { }
 
 lemma lemma_fundamental_div_mod(x:int, d:int)
-    requires d != 0;
-    ensures x == d * (x/d) + (x%d);
+  requires d != 0
+  ensures x == d * (x/d) + (x%d)
 { }
 
 lemma lemma_0_mod_anything()
-    ensures forall m:int {:trigger 0 % m} :: m > 0 ==> 0 % m == 0;
+  ensures forall m:int {:trigger 0 % m} :: m > 0 ==> 0 % m == 0
 { }
 
 // lemma lemma_mod_yourself(m:int)
-//     ensures m > 0 ==> m % m == 0;
+//   ensures m > 0 ==> m % m == 0
 // { }
 
 lemma lemma_small_mod(x:nat, m:nat)
-    requires x<m;
-    requires 0<m;
-    ensures x % m == x;
+  requires x<m
+  requires 0<m
+  ensures x % m == x
 { }
 
 lemma lemma_mod_range(x:int, m:int)
-    requires m > 0;
-    ensures 0 <= x % m < m;
+  requires m > 0
+  ensures 0 <= x % m < m
 { }
 
 lemma lemma_real_div_gt(x:real, y:real)
-    requires x > y;
-    requires x >= 0.0;
-    requires y > 0.0;
-    ensures  x / y > real(1);
+  requires x > y
+  requires x >= 0.0
+  requires y > 0.0
+  ensures  x / y > 1 as real
 { }
 
 } 
